promising-arm/VMPromising.v
@@ -1,0 +1,1071 @@
+
+Require Import Strings.String.
+Require Import SSCCommon.Common.
+Require Import SSCCommon.Exec.
+Require Import Coq.Program.Equality.
+
+From stdpp Require Import decidable.
+From stdpp Require Import pretty.
+
+Require UMPromising.
+
+Require Import ISASem.ArmInst.
+Require Import GenModels.TermModels.
+Import UMPromising.TM.
+Require Import GenPromising.
+Import UMPromising.GP.
+
+(** The goal of this module is to define an Virtual memory promising model,
+    without mixed-size on top of the new interface *)
+
+(** This model only works for 8-bytes aligned locations, as there
+    in no support for mixed-sizes yet. Also all location are
+    implicitly in the non-secure world.
+
+    So in order to get the physical address you need to append 3 zeros.
+
+    We reuse the location setup from the User-Mode promising model. *)
+Module Loc := UMPromising.Loc.
+
+(** Register and memory values (all memory access are 8 bytes aligned *)
+Definition val := bv 64.
+
+
+(** We also reuse the Msg object from the User-Mode Promising Model. *)
+Module Msg := UMPromising.Msg.
+
+Module TLBI.
+  Inductive t :=
+  | All (tid : nat)
+  | Asid (tid : nat) (asid : bv 16)
+  | Va (tid : nat) (asid : bv 16) (va : bv 36) (last : bool)
+  | Vaa (tid : nat) (va : bv 36) (last : bool).
+
+  #[global] Instance dec : EqDecision t.
+  solve_decision.
+  Defined.
+
+  Definition tid (tlbi : t) : nat :=
+    match tlbi with
+    | All tid => tid
+    | Asid tid _ => tid
+    | Va tid _ _ _ => tid
+    | Vaa tid _ _ => tid
+    end.
+
+  Definition asid_opt (tlbi : t) : option (bv 16) :=
+    match tlbi with
+    | All _ => None
+    | Asid _ asid => Some asid
+    | Va _ asid _ _ => Some asid
+    | Vaa _ _ _ => None
+    end.
+
+  Definition asid (tlbi : t) : bv 16 :=
+    default (Z_to_bv 16 0) (asid_opt tlbi).
+
+  Definition va_opt (tlbi : t) : option (bv 36) :=
+    match tlbi with
+    | All _ => None
+    | Asid _ _ => None
+    | Va _ _ va _ => Some va
+    | Vaa _ va _ => Some va
+    end.
+
+  Definition va (tlbi : t) : bv 36 :=
+    default (Z_to_bv 36 0) (va_opt tlbi).
+
+  Definition last_opt (tlbi : t) : option bool :=
+    match tlbi with
+    | All _ => None
+    | Asid _ _ => None
+    | Va _ _ _ last => Some last
+    | Vaa _ _ last => Some last
+    end.
+
+  Definition last (tlbi : t) : bool :=
+    default false (last_opt tlbi).
+End TLBI.
+
+(** Promising events appearing in the trace *)
+Module Ev.
+  Inductive t :=
+  | Msg (msg : Msg.t)
+  | Tlbi (tlbi : TLBI.t).
+
+  #[global] Instance dec : EqDecision t.
+  solve_decision.
+  Defined.
+
+  Definition tid (ev : t) :=
+    match ev with
+    | Msg msg => Msg.tid msg
+    | Tlbi tlbi => TLBI.tid tlbi
+    end.
+
+  Definition is_write_to (loc : Loc.t) (ev : t) :=
+    match ev with
+    | Msg msg => Msg.loc msg =? loc
+    | Tlbi _ => false
+    end.
+End Ev.
+Coercion Ev.Msg : Msg.t >-> Ev.t.
+Coercion Ev.Tlbi : TLBI.t >-> Ev.t.
+
+
+(** A view is just a natural *)
+Definition view := nat.
+Bind Scope nat_scope with view.
+Global Hint Transparent view : core.
+Global Hint Unfold view : core.
+
+Module Memory.
+  Import PromMemory.
+
+  (** Representation of initial memory, this is representation
+      optimized for the internals of this model, so it not a plain
+      memoryMap *)
+  Definition initial := Loc.t -> val.
+
+  (** Convert from a memoryMap to the internal representation: initial *)
+  Definition initial_from_memMap (mem : memoryMap) : initial :=
+    fun loc => Loc.to_pas loc |> map mem |> bv_of_bytes 8 64.
+
+  (** The promising memory: a list of events *)
+  Definition t : Type := t Ev.t.
+
+  Definition cut_after : nat -> t -> t := @cut_after Ev.t.
+  Definition cut_before : nat -> t -> t := @cut_before Ev.t.
+
+
+
+ (** Reads the last write to a location in some memory. Gives the value and the
+     timestamp of the write that it read from.
+     The timestamp is 0 if reading from initial memory. *)
+  Fixpoint read_last (loc : Loc.t) (init : initial) (mem : t) : (val * nat) :=
+    match mem with
+    | [] => (init loc, 0%nat)
+    | (Ev.Msg msg) :: mem' =>
+        if Msg.loc msg =? loc then
+          (Msg.val msg, List.length mem)
+        else read_last loc init mem'
+    | Ev.Tlbi _ :: mem' => read_last loc init mem'
+    end.
+
+  (** Reads from initial memory and fail if the memory has been overwritten.
+
+      This is mainly for instruction fetching in this model *)
+  Definition read_initial (loc : Loc.t) (init : initial) (mem : t) : option val :=
+    match read_last loc init mem with
+    | (v, 0%nat) => Some v
+    | _ => None
+    end.
+
+  (* (** Reads from initial memory for instruction fetch (only 4 bytes aligned) *)
+  (*     and fail if the memory was modified *)
+  (*  *) *)
+  (* Definition read_ifetch (addr : bv 50) (init : initial) (mem : t) *)
+  (*   : option val := *)
+  (*   if existsb (fun ev => *)
+  (*                 match ev with *)
+  (*                 | Ev.Msg msg => Msg.lov msg =? (bv_extract 1 49 addr) *)
+  (*                 | _ => false) mem *)
+  (*   then None *)
+  (*   else Some ( *)
+  (*   match read_last loc init mem with *)
+  (*   | (v, 0%nat) => Some v *)
+  (*   | _ => None *)
+  (*   end. *)
+
+
+
+  (** To a snapshot of the memory back to a memoryMap *)
+  Definition to_memMap (init : initial) (mem : t) : memoryMap:=
+    fun pa =>
+      (loc ← Loc.from_pa_in pa;
+      let '(v, _) := read_last loc init mem in
+      index ← Loc.pa_index pa;
+      bv_to_bytes 8 v !! bv_unsigned index)
+        |> default (bv_0 8).
+
+  (** Adds the view number to each message given a view for the last message.
+      This is for convenient use with cut_after.
+
+      TODO: it would make sense to make a function that does cut_after
+      and this in a single step. *)
+  (* Fixpoint with_views_from (v : view) (mem : t) *)
+  (*   : list (Msg.t * view) := *)
+  (*   match mem with *)
+  (*   | [] => [] *)
+  (*   | h :: q => (v, h) :: with_views_from (v - 1) q *)
+  (*   end. *)
+
+
+  (** Returns the list of possible reads at a location restricted by a certain
+      view. The list is never empty as one can always read from at least the
+      initial value. *)
+  Definition read (loc : Loc.t) (v : view) (init : initial) (mem : t)
+    : list (val * view) :=
+    let first := mem |> cut_before v |> read_last loc init in
+    let lasts := mem |> cut_after_with_timestamps v
+                     |> list_filter_map
+                     (fun '(ev, v) =>
+                        match ev with
+                        | Ev.Msg msg =>
+                            if Msg.loc msg =? loc
+                            then Some (Msg.val msg, v)
+                            else None
+                        | Ev.Tlbi _ => None
+                        end)
+    in
+    lasts ++ [first].
+
+  (** Promise a write and add it at the end of memory *)
+  Definition promise (ev : Ev.t) (mem : t) : view * t :=
+    let nmem := ev :: mem in (List.length nmem, nmem).
+
+  (** Returns a view among a promise set that correspond to an event. The
+      oldest matching view is taken. This is because it can be proven that
+      taking a more recent view, will make the previous promises unfulfillable
+      and thus the corresponding executions would be discarded. TODO prove it.
+      *)
+  Definition fulfill (ev : Ev.t) (prom : list view) (mem : t) : option view :=
+    prom |> filter (fun t => Some ev =? mem !! t)
+         |> reverse
+         |> head.
+
+  (** Check that the write at the provided timestamp is indeed to that location
+      and that no write to that location have been made by any other thread *)
+  Definition exclusive (loc : Loc.t) (v : view) (mem : t) : bool:=
+    match mem !! v with
+    | Some (Ev.Msg msg) =>
+        if Msg.loc msg =? loc then
+          let tid := Msg.tid msg in
+          mem |> cut_after v
+              |> forallb
+              (fun ev => match ev with
+                      | Ev.Msg msg =>
+                          (Msg.tid msg =? tid)
+                          || negb (Msg.loc msg =? loc)
+                      | _ => true
+                      end)
+        else false
+    | _ => false
+    end.
+
+End Memory.
+
+Module FwdItem.
+   Record t :=
+    make {
+        time : nat;
+        view : view;
+        xcl : bool
+      }.
+
+   Definition init := make 0 0 false.
+End FwdItem.
+
+(* Python:
+for i in range(11, 31):
+    print("Notation \"{}\" := (FS {}) : fin_scope.".format(i, i - 1))
+*)
+Notation "11" := (FS 10) : fin_scope.
+Notation "12" := (FS 11) : fin_scope.
+Notation "13" := (FS 12) : fin_scope.
+Notation "14" := (FS 13) : fin_scope.
+Notation "15" := (FS 14) : fin_scope.
+Notation "16" := (FS 15) : fin_scope.
+Notation "17" := (FS 16) : fin_scope.
+Notation "18" := (FS 17) : fin_scope.
+Notation "19" := (FS 18) : fin_scope.
+Notation "20" := (FS 19) : fin_scope.
+Notation "21" := (FS 20) : fin_scope.
+Notation "22" := (FS 21) : fin_scope.
+Notation "23" := (FS 22) : fin_scope.
+Notation "24" := (FS 23) : fin_scope.
+Notation "25" := (FS 24) : fin_scope.
+Notation "26" := (FS 25) : fin_scope.
+Notation "27" := (FS 26) : fin_scope.
+Notation "28" := (FS 27) : fin_scope.
+Notation "29" := (FS 28) : fin_scope.
+Notation "30" := (FS 29) : fin_scope.
+
+
+Bind Scope fin_scope with fin.
+Definition EL := (fin 4).
+Bind Scope fin_scope with EL.
+Definition ELp := (fin 3).
+Bind Scope fin_scope with ELp.
+
+
+Bind Scope string_scope with reg.
+
+Definition ELp_to_EL : ELp -> EL := FS.
+
+Global Instance pretty_fin (n : nat) : Pretty (fin n)  :=
+  (fun n => pretty (n : nat)).
+Global Hint Mode Pretty ! : typeclass_instances.
+
+
+(** Any write to a register not explicitly supported by Reg.t will fail,
+    because this means that the model doesn't know which behavior it is supposed to
+    have *)
+Module Reg.
+  (** application registers *)
+  Inductive app :=
+  | R (num : fin 31)
+  | SP (el : EL).
+
+  #[global] Instance app_dec : EqDecision app.
+  solve_decision.
+  Defined.
+
+  Inductive sys :=
+  | ELR (el : ELp)
+  | FAR (el : ELp)
+  | PAR (* EL1 *)
+  | TTBR0 (el : ELp)
+  | TTBR1_EL1
+  | TTBR1_EL2
+  | VBAR (el : ELp)
+  | VTTBR (* EL2 *).
+
+  #[global] Instance sys_dec : EqDecision sys.
+  solve_decision.
+  Defined.
+
+
+  Inductive t :=
+  | App (app : app)
+  | Sys (sys : sys).
+
+  #[global] Instance dec : EqDecision t.
+  solve_decision.
+  Defined.
+
+  (* TODO generate that automatically? *)
+  Definition from_arch (r : reg) :=
+    match r with
+    | "R0" => Some (App (R 0))
+    | "R1" => Some (App (R 1))
+    | "R2" => Some (App (R 2))
+    | "R3" => Some (App (R 3))
+    | "R4" => Some (App (R 4))
+    | "R5" => Some (App (R 5))
+    | "R6" => Some (App (R 6))
+    | "R7" => Some (App (R 7))
+    | "R8" => Some (App (R 8))
+    | "R9" => Some (App (R 9))
+    | "R10" => Some (App (R 10))
+    | "R11" => Some (App (R 11))
+    | "R12" => Some (App (R 12))
+    | "R13" => Some (App (R 13))
+    | "R14" => Some (App (R 14))
+    | "R15" => Some (App (R 15))
+    | "R16" => Some (App (R 16))
+    | "R17" => Some (App (R 17))
+    | "R18" => Some (App (R 18))
+    | "R19" => Some (App (R 19))
+    | "R20" => Some (App (R 20))
+    | "R21" => Some (App (R 21))
+    | "R22" => Some (App (R 22))
+    | "R23" => Some (App (R 23))
+    | "R24" => Some (App (R 24))
+    | "R25" => Some (App (R 25))
+    | "R26" => Some (App (R 26))
+    | "R27" => Some (App (R 27))
+    | "R28" => Some (App (R 28))
+    | "R29" => Some (App (R 29))
+    | "R30" => Some (App (R 30))
+    | "SP_EL0" => Some (App (SP 0))
+    | "SP_EL1" => Some (App (SP 1))
+    | "SP_EL2" => Some (App (SP 2))
+    | "SP_EL3" => Some (App (SP 3))
+    | "ELR_EL1" => Some (Sys (ELR 0))
+    | "ELR_EL2" => Some (Sys (ELR 1))
+    | "ELR_EL3" => Some (Sys (ELR 2))
+    | "FAR_EL1" => Some (Sys (FAR 0))
+    | "FAR_EL2" => Some (Sys (FAR 1))
+    | "FAR_EL3" => Some (Sys (FAR 2))
+    | "PAR_EL1" => Some (Sys PAR)
+    | "TTBR0_EL1" => Some (Sys (TTBR0 0))
+    | "TTBR0_EL2" => Some (Sys (TTBR0 1))
+    | "TTBR0_EL3" => Some (Sys (TTBR0 2))
+    | "TTBR1_EL1" => Some (Sys TTBR1_EL1)
+    | "TTBR1_EL2" => Some (Sys TTBR1_EL2)
+    | "VBAR_EL1" => Some (Sys (VBAR 0))
+    | "VBAR_EL2" => Some (Sys (VBAR 1))
+    | "VBAR_EL3" => Some (Sys (VBAR 2))
+    | "VTTBR_EL2" => Some (Sys VTTBR)
+    | _ => None
+    end.
+
+  Definition to_arch (reg : t) : Inst.reg :=
+    match reg with
+    | App (R n) => "R" ++ (pretty n)
+    | App (SP n) => "SP_EL" ++ (pretty n)
+    | Sys (ELR n) => "ELR_EL" ++ (pretty (S n))
+    | Sys (FAR n) => "FAR_EL" ++ (pretty (S n))
+    | Sys PAR => "PAR_EL1"
+    | Sys (TTBR0 n) => "TTBR0_EL" ++ (pretty (S n))
+    | Sys TTBR1_EL1 => "TTBR1_EL1"
+    | Sys TTBR1_EL2 => "TTBR1_EL2"
+    | Sys (VBAR n) => "VBAR_EL" ++ (pretty (S n))
+    | Sys VTTBR => "VTTBR_EL2"
+    end.
+
+
+  Ltac fin_case :=
+    match goal with
+    | n : fin 0 |- _ => dep_destruct n
+    | n : fin _ |- _ => dep_destruct n; [| clear n]
+    end.
+
+  Lemma to_from_arch (reg : t) : from_arch (to_arch reg) = Some reg.
+  Proof.
+    destruct reg as [app | sys].
+    - destruct app;
+        unfold EL in *;
+        repeat (fin_case; [sfirstorder |]);
+        try (fin_case).
+    - destruct sys;
+        unfold ELp in *;
+        repeat (fin_case; [sfirstorder |]);
+        try (fin_case);
+        sfirstorder.
+  Qed.
+
+  Lemma from_to_arch (r : reg) (r' : t) : (from_arch r) = Some r' -> to_arch r' = r.
+  Proof.
+    intro H.
+    unfold from_arch in H.
+    (* takes around 2s *)
+    repeat (discriminate H || case_split); inversion H; vm_compute; reflexivity.
+  Qed.
+
+End Reg.
+Coercion Reg.App : Reg.app >-> Reg.t.
+Coercion Reg.Sys : Reg.sys >-> Reg.t.
+
+Module WSReg.
+  Record t :=
+    make {
+        sreg : Reg.sys;
+        val : regval;
+        view : nat
+      }.
+
+
+  Definition to_val_view (wsreg : t) := (wsreg.(val), wsreg.(view)).
+End WSReg.
+
+
+
+(** The thread state *)
+Module TState.
+  Record t :=
+    make {
+        (* The promises that this thread must fullfil
+           Is must be ordered with oldest promises at the bottom of the list *)
+        prom : list view;
+
+        (* registers values and views *)
+        regs : Reg.app -> regval * view;
+        regs_init : registerMap;
+        sregs : list WSReg.t;
+
+        (* The coherence views *)
+        coh : Loc.t -> view;
+
+
+        vrd : view; (* The maximum output view of a read  *)
+        vwr : view; (* The maximum output view of a write  *)
+        vdmbst : view; (* The maximum output view of a dmb st  *)
+        vdmb : view; (* The maximum output view of a dmb ld or dmb sy  *)
+        vdsb : view; (* The maximum output view of a dsb  *)
+        vspec : view; (* The maximum output view of speculative operation. *)
+        vcse : view; (* The maximum output view of an Context Synchronization Event *)
+        vtlbi : view; (* The maximum output view of an TLBI *)
+        vmsr : view; (* The maximum output view of an MSR *)
+        vacq : view; (* The maximum output view of an acquire access *)
+        vrel : view; (* The maximum output view of an release access *)
+
+        (* Forwarding database. The first view is the timestamp of the
+           write while the second view is the max view of the dependencies
+           of the write. The boolean marks if the store was an exclusive*)
+        fwdb : Loc.t -> FwdItem.t;
+
+        (* Exclusive database. If there was a recent load exclusive but the
+           corresponding store exclusive has not yet run, this will contain
+           the timestamp and post-view of the load exclusive*)
+        xclb : option (nat * view);
+
+        (* Position in sregs of the last CSE event *)
+        scse : nat;
+
+        (* Recording of all previous updates of the MMU/TLB view of the system
+           registers *)
+        tlbscses : nat -> option nat
+      }.
+
+  #[global] Instance eta : Settable _ :=
+    settable! make <prom;regs;regs_init;sregs;coh;vrd;vwr;vdmbst;vdmb;vdsb;
+                    vspec;vcse;vtlbi;vmsr;vacq;vrel;fwdb;xclb;scse;tlbscses>.
+
+  Definition init (mem : memoryMap) (iregs : registerMap) :=
+    ({|
+      prom := [];
+      regs := fun reg => (iregs (Reg.to_arch reg), 0);
+      regs_init := iregs;
+      sregs := [];
+      coh := fun loc => 0;
+      vrd := 0;
+      vwr := 0;
+      vdmbst := 0;
+      vdmb := 0;
+      vdsb := 0;
+      vspec := 0;
+      vcse := 0;
+      vtlbi := 0;
+      vmsr := 0;
+      vacq := 0;
+      vrel := 0;
+      fwdb := fun loc => FwdItem.init;
+      xclb := None;
+      scse := 0;
+      tlbscses := (fun _ => None)
+    |})%nat.
+
+  Definition sreg_cur (ts : t) := length ts.(sregs).
+
+  (** Read the last system register write at system register position s *)
+  Definition read_sreg_last (ts : t) (s : nat) (sreg : Reg.sys) :=
+    ts.(sregs)
+         |> drop ((sreg_cur ts) - s)
+         |> filter (fun wsreg => wsreg.(WSReg.sreg) = sreg)
+         |> hd_error
+         |> fmap (M:= option) WSReg.to_val_view
+         |> default (ts.(regs_init) (Reg.to_arch sreg), 0%nat).
+
+  (** Read all possible system register values for sreg assuming the last
+      synchronization at position sync *)
+  Definition read_sreg (ts : t) (sync : nat) (sreg : Reg.sys)
+    : list (regval * view)
+    :=
+    let rest :=
+      ts.(sregs)
+           |> take ((sreg_cur ts) - sync)
+           |> filter (fun wsreg => wsreg.(WSReg.sreg) = sreg)
+           |> map WSReg.to_val_view
+    in (read_sreg_last ts sync sreg) :: rest.
+
+  (** Read uniformly a register of any kind. *)
+  Definition read_reg (ts : t) (r : reg) : regval * view :=
+    match Reg.from_arch r with
+    | Some (Reg.App app) => ts.(regs) app
+    | Some (Reg.Sys sys) => read_sreg_last ts (sreg_cur ts) sys
+    | None => (ts.(regs_init) r, 0%nat)
+    end.
+
+  (** Extract a plain register map from the thread state without views.
+      This is used to decide if a thread has terminated, and to observe the
+      results of the model *)
+  Definition reg_map (ts : t) : registerMap := fst ∘ read_reg ts.
+
+  (** Sets the value of a register *)
+  Definition set_reg (reg : Reg.app) (rv : reg_type * view) : t -> t
+    := set regs (fun_add reg rv).
+
+  (** Sets the coherence view of a location *)
+  Definition set_coh (loc : Loc.t) (v : view) : t -> t :=
+    set coh (fun_add loc v).
+
+  (** Updates the coherence view of a location by taking the max of the new
+      view and of the existing value *)
+  Definition update_coh (loc : Loc.t) (v : view) (s : t) : t :=
+    set_coh loc (max v (coh s loc)) s.
+
+  (** Updates the forwarding database for a location. *)
+  Definition set_fwdb (loc : Loc.t) (fi : FwdItem.t) : t -> t :=
+    set fwdb (fun_add loc fi).
+
+  (** Set the exclusive database to the timestamp and view of the latest
+      load exclusive *)
+  Definition set_xclb (vs : view * view) : t -> t :=
+    set xclb (fun _ => Some vs).
+
+  (** Clear the exclusive database, to mark a store exclusive *)
+  Definition clear_xclb : t -> t :=
+    set xclb (fun _ => None).
+
+  (** Updates a view that from the state, by taking the max of new value and
+      the current value.
+
+      For example `update rmax vnew t` does t.rmax <- max t.rmax vnew *)
+  Definition update (acc : t -> view) {_: Setter acc}
+             (v : view) : t -> t :=
+    set acc (max v).
+
+  (** Updates two view in the same way as update. Purely for convenience *)
+  Definition update2 (acc1 acc2 : t -> view) {_: Setter acc1} {_: Setter acc2}
+             (v : view) : t -> t :=
+    (update acc1 v) ∘ (update acc2 v).
+
+  (** Add a promise to the promise set *)
+  Definition promise (v : view) : t -> t := set prom (fun p => v :: p).
+
+  (** Perform a context synchronization event *)
+  Definition cse (v : view) (ts : t) : t :=
+    ts |> setv scse (length ts.(sregs))
+       |> update vcse v.
+End TState.
+
+
+(*** Instruction semantics ***)
+
+(** Intra instruction state for propagating views inside an instruction *)
+Module IIS.
+
+  (* Translation Results *)
+  Module TransRes.
+    Record t :=
+      make {
+          time : nat;
+          remaining : list (bv 64);
+          invalidation : nat
+        }.
+
+    #[global] Instance eta : Settable _ :=
+      settable! make <time; remaining; invalidation>.
+
+    Definition pop (tr : t) : Exec.t string (bv 64 * t) :=
+      match tr.(remaining) with
+      | h :: tl => Exec.ret (h, setv remaining tl tr)
+      | _ => Exec.Error
+              "Couldn't pop the next PTE: error in translation assumptions"
+      end.
+  End TransRes.
+
+  Record t :=
+    make {
+        regs : view; (* All the register reads that happened before *)
+        nreg : view;(* All the previous non-register events *)
+        reads : list view; (* The post view of all the reads *)
+        (* The translations whose results were already selected *)
+        trs : bv 36 -> option TransRes.t
+      }.
+
+  #[global] Instance eta : Settable _ :=
+    settable! make <regs;nreg;reads; trs>.
+
+  Definition init : t := make 0 0 [] (fun _ => None).
+
+  (** Add a new memory read to the IIS *)
+  Definition add_read (v : view) (iis : t) : t :=
+    iis |> set nreg (max v)
+        |> set reads (.++ [v]).
+
+  (** Add a new non-register event to the IIS *)
+  Definition add_nreg (v : view) (iis : t) : t :=
+    iis |> set nreg (max v).
+
+  (** Add a new register read to the IIS *)
+  Definition add_reg (v : view) (iis : t) : t :=
+    iis |> set regs (max v).
+
+  Definition from_read_deps (deps : list N) (iis : t) : view :=
+   List.fold_left (fun v dep => match iis.(reads) !! dep with
+                                  | Some v' => max v v'
+                                  | None => v end) deps 0%nat.
+
+  Definition from_DepOn (deps : DepOn.t) (ts : TState.t) (iis : t)
+    : view :=
+    max (from_read_deps deps.(DepOn.mem_reads) iis) $
+    List.fold_left (fun v reg => max v $ snd $ TState.read_reg ts reg)
+                   deps.(DepOn.regs) 0%nat.
+
+  Definition from_DepOn_opt (deps : option DepOn.t) regsm iis :=
+    match deps with
+    | None => iis.(regs) ⊔ list_max iis.(reads)
+    | Some deps => from_DepOn deps regsm iis
+    end.
+
+  Definition set_trs (va : bv 36) (tres : TransRes.t) :=
+    set trs (fun_add va (Some tres)).
+
+End IIS.
+
+
+Definition view_if (b : bool) (v : view) := if b then v else 0%nat.
+
+(** The view of a read from a forwarded write *)
+Definition read_fwd_view (ak : Explicit_access_kind) (f : FwdItem.t) :=
+  if f.(FwdItem.xcl) && negb (ak.(Explicit_access_kind_strength) =? AS_normal)
+  then f.(FwdItem.time) else f.(FwdItem.view).
+
+(*** VA helper ***)
+
+Definition prefix_to_va {n : N} (p : bv n) : bv 64 :=
+  bv_concat 64 (bv_0 16) (bv_concat 48 p (bv_0 (48 - n))).
+
+Definition level_prefix {n : N} (va : bv n) (lvl : N) :=
+  bv_extract (12 + 9 * (3 - lvl)) (9 * (lvl + 1)) va.
+
+Definition level_index {n : N} (va : bv n) (lvl : N) : bv 9 :=
+  bv_extract 0 9 (level_prefix va lvl).
+
+Definition higher_level {n : N} (va : bv n) : bv (n - 9) :=
+  bv_extract 9 (n - 9) va.
+
+Definition next_entry_loc (loc : Loc.t) (index : bv 9) : Loc.t :=
+  bv_concat 49 (bv_extract 9 40 loc) index.
+
+
+(** Performs a memory read at a location with a view and return possible output
+    states with the timestamp and value of the read *)
+Definition read_mem_explicit (loc : Loc.t) (vaddr : view) (viio : view)
+  (invalidation_time : nat) (ak : Explicit_access_kind) (ts : TState.t)
+  (init : Memory.initial) (mem : Memory.t)
+  : Exec.t string (TState.t * view * val) :=
+  let acs := ak.(Explicit_access_kind_strength) in
+  let acv := ak.(Explicit_access_kind_variety) in
+  Exec.fail_if (acv =? AV_atomic_rmw) "Atomic RMV unsupported";;
+  let vbob := ts.(TState.vdmb) ⊔ ts.(TState.vdsb)
+              ⊔ ts.(TState.vcse) ⊔ ts.(TState.vacq)
+                (* Strong Acquire loads are ordered after Release stores *)
+              ⊔ view_if (acs =? AS_rel_or_acq) ts.(TState.vrel) in
+  let vpre := vaddr ⊔ vbob ⊔ viio in
+  (* We only read after the coherence point, because without mixed-size, this
+     is equivalent to reading at vpre and discarding incoherent options *)
+  let vread := vpre ⊔ (TState.coh ts loc) in
+  '(res, time) ← Exec.Results $ Memory.read loc vread init mem;
+  let fwd := TState.fwdb ts loc in
+  let read_view :=
+    if (fwd.(FwdItem.time) =? time) then read_fwd_view ak fwd else time in
+  let vpost := vpre ⊔ read_view in
+  Exec.assert (vpost <=? invalidation_time)%nat;;
+  let ts :=
+    ts |> TState.update_coh loc time
+       |> TState.update TState.vrd vpost
+       |> TState.update TState.vacq (view_if (negb (acs =? AS_normal)) vpost)
+       |> TState.update TState.vspec vaddr
+       |> (if acv =? AV_exclusive then TState.set_xclb (time, vpost) else id)
+  in Exec.ret (ts, vpost, res).
+
+Definition read_pte (ts : TState.t) (vaddr : view) (viio : view)
+  (tsum : translation) (tres : IIS.TransRes.t)
+  : Exec.t string (TState.t * view * val * IIS.TransRes.t) :=
+  let vpost := vaddr ⊔ viio ⊔ tres.(IIS.TransRes.time) in
+  '(val, tres) ← IIS.TransRes.pop tres;
+  let ts := ts |> TState.update TState.vspec vpost in
+  Exec.ret (ts, vpost, val, tres).
+
+
+
+
+(** Run a MemRead outcome.
+    Returns the new thread state, the vpost of the read and the read value. *)
+Definition run_mem_read (rr : ReadReq.t 8) (iis : IIS.t)
+  (ts : TState.t) (init : Memory.initial) (mem : Memory.t)
+  : Exec.t string (TState.t * IIS.t * val) :=
+  addr ← Exec.error_none "PA not supported" $ Loc.from_pa rr.(ReadReq.pa);
+  let vaddr :=
+    IIS.from_DepOn_opt rr.(ReadReq.addr_dep_on) ts iis
+  in
+  let va : bv 64 := default (Loc.to_va addr) rr.(ReadReq.va) in
+  let trans_res := iis.(IIS.trs) (bv_extract 12 36 va) in
+  let inv :=
+    trans_res |> fmap (fun tr => tr.(IIS.TransRes.invalidation)) |> default (0 % nat)
+  in
+  let viio := IIS.nreg iis in
+  match rr.(ReadReq.access_kind) with
+  | AK_explicit eak =>
+      '(ts, view, val) ← read_mem_explicit addr vaddr viio inv eak ts init mem;
+      let iis := IIS.add_read view iis in
+      Exec.ret (ts, iis, val)
+  | AK_ttw () =>
+      tres ← Exec.error_none "TTW read before translation start" trans_res;
+      '(ts, view, val, tres) ←
+        read_pte ts vaddr viio rr.(ReadReq.translation) tres;
+      let iis :=
+        iis |> IIS.add_read view
+          |> IIS.set_trs (bv_extract 12 36 va) tres
+      in Exec.ret (ts, iis, val)
+  | AK_ifetch () => Exec.Error "8 bytes ifetch ???"
+  | _ => Exec.Error "Only ifetch, ttw and explicit accesses supported"
+  end.
+
+
+Definition run_mem_read4 (rr : ReadReq.t 4) (iis : IIS.t)
+  (ts : TState.t) (init : Memory.initial) (mem : Memory.t)
+  : Exec.t string (bv 32) :=
+  let addr := rr.(ReadReq.pa) in
+  let aligned_addr := set FullAddress_address (bv_unset_bit 2) addr in
+  let bit2 := addr.(FullAddress_address) |> bv_get_bit 2 in
+  loc ← Exec.error_none "PA not supported" $ Loc.from_pa aligned_addr;
+  match rr.(ReadReq.access_kind) with
+  | AK_ifetch () =>
+      block ← Exec.error_none "Modified instruction memory"
+                              (Memory.read_initial loc init mem);
+      (if bit2 then bv_extract 32 32 else bv_extract 0 32) block
+        |> Exec.ret
+  | _ => Exec.Error "4 bytes accesses unsupported (except ifetch)"
+  end.
+
+
+
+(** Performs a memory write for a thread tid at a location loc with view
+    vaddr and vdata. Return the new state.
+
+    This may mutate memory if no existing promise can be fullfilled *)
+Definition write_mem (tid : nat) (loc : Loc.t) (vaddr : view) (vdata : view)
+           (viio : view)
+           (acs : Access_strength) (ts : TState.t) (mem : Memory.t)
+           (data : val) : Exec.t string (TState.t * Memory.t * view):=
+  let msg := Msg.make tid loc data in
+  let is_release := acs =? AS_rel_or_acq in
+  let '(time, mem) :=
+    match Memory.fulfill msg (TState.prom ts) mem with
+    | Some t => (t, mem)
+    | None => Memory.promise msg mem
+    end in
+  let vbob :=
+    ts.(TState.vdmbst) ⊔ ts.(TState.vdmb) ⊔ ts.(TState.vdsb)
+    ⊔ ts.(TState.vcse) ⊔ ts.(TState.vacq)
+    ⊔ view_if is_release (ts.(TState.vrd) ⊔ ts.(TState.vwr)) in
+  let vpre := vaddr ⊔ vdata ⊔ ts.(TState.vspec) ⊔ vbob ⊔ viio in
+  Exec.assert (vpre ⊔ (TState.coh ts loc) <? time)%nat;;
+  let ts :=
+    ts |> set TState.prom (delete time)
+       |> TState.update_coh loc time
+       |> TState.update TState.vwr time
+       |> TState.update TState.vrel (view_if is_release time)
+       |> TState.update TState.vspec vaddr
+  in Exec.ret (ts, mem, time).
+
+
+(** Tries to perform a memory write.
+
+    If the store is not exclusive, the write is always performed and the third
+    return value is true.
+
+    If the store is exclusive the write may succeed or fail and the third
+    return value indicate the success (true for success, false for error) *)
+Definition write_mem_xcl (tid : nat) (loc : Loc.t) (vaddr : view)
+           (vdata : view) (viio : view) (ak : Explicit_access_kind)
+           (ts : TState.t) (mem : Memory.t) (data : val)
+  : Exec.t string (TState.t * Memory.t):=
+  let acs := Explicit_access_kind_strength ak in
+  let acv := Explicit_access_kind_variety ak in
+  Exec.fail_if (acv =? AV_atomic_rmw) "Atomic RMV unsupported";;
+  let xcl := acv =? AV_exclusive in
+  if xcl then
+    '(ts, mem, time) ← write_mem tid loc vaddr vdata viio acs ts mem data;
+    match TState.xclb ts with
+    | None => Exec.discard
+    | Some (xtime, xview) =>
+        Exec.assert $ Memory.exclusive loc xtime (Memory.cut_after time mem)
+    end;;
+    let ts := TState.set_fwdb loc (FwdItem.make time (vaddr ⊔ vdata) true) ts in
+    Exec.ret (TState.clear_xclb ts, mem)
+  else
+    '(ts, mem, time) ← write_mem tid loc vaddr vdata viio acs ts mem data;
+    let ts := TState.set_fwdb loc (FwdItem.make time (vaddr ⊔ vdata) false) ts in
+    Exec.ret (ts, mem).
+
+
+(** Perform a barrier, mostly view shuffling *)
+Definition run_barrier (iis : IIS.t) (ts : TState.t) (barrier : barrier) :
+  Exec.t string (IIS.t * TState.t) :=
+  match barrier with
+  | Barrier_DMB dmb => (* dmb *)
+       match dmb.(DxB_types) with
+      | MBReqTypes_All (* dmb sy *) =>
+          let vpost :=
+            ts.(TState.vrd) ⊔ ts.(TState.vwr)
+            ⊔ ts.(TState.vcse) ⊔ ts.(TState.vdsb)
+          in
+          Exec.ret (IIS.add_nreg vpost iis, TState.update TState.vdmb vpost ts)
+      | MBReqTypes_Reads (* dmb ld *) =>
+          let vpost := ts.(TState.vrd) ⊔ ts.(TState.vcse) ⊔ ts.(TState.vdsb) in
+          Exec.ret (IIS.add_nreg vpost iis, TState.update TState.vdmb vpost ts)
+      | MBReqTypes_Writes (* dmb st *) =>
+          let vpost := ts.(TState.vwr) ⊔ ts.(TState.vcse) ⊔ ts.(TState.vdsb) in
+          Exec.ret (IIS.add_nreg vpost iis, TState.update TState.vdmbst vpost ts)
+      end
+  | Barrier_DSB dmb => (* dsb *)
+      Exec.fail_if (dmb.(DxB_domain) =? MBReqDomain_Nonshareable)
+        "Non-shareable barrier are not supported";;
+       match dmb.(DxB_types) with
+      | MBReqTypes_All (* dsb sy *) =>
+          let vpost :=
+            ts.(TState.vrd) ⊔ ts.(TState.vwr)
+            ⊔ ts.(TState.vdmb) ⊔ ts.(TState.vdmbst)
+            ⊔ ts.(TState.vcse) ⊔ ts.(TState.vdsb) ⊔ ts.(TState.vtlbi)
+          in
+          Exec.ret (IIS.add_nreg vpost iis, TState.update TState.vdsb vpost ts)
+      | MBReqTypes_Reads (* dsb ld *) =>
+          let vpost := ts.(TState.vrd) ⊔ ts.(TState.vcse) ⊔ ts.(TState.vdsb) in
+          Exec.ret (IIS.add_nreg vpost iis, TState.update TState.vdsb vpost ts)
+      | MBReqTypes_Writes (* dsb st *) =>
+          let vpost := ts.(TState.vwr) ⊔ ts.(TState.vcse) ⊔ ts.(TState.vdsb) in
+          Exec.ret (IIS.add_nreg vpost iis, TState.update TState.vdsb vpost ts)
+      end
+  | Barrier_ISB () => (* isb *)
+      let vpost :=
+        ts.(TState.vspec) ⊔ ts.(TState.vcse)
+        ⊔ ts.(TState.vdsb) ⊔ ts.(TState.vmsr)
+      in
+      Exec.ret (IIS.add_nreg vpost iis, TState.cse vpost ts)
+  | _ => Exec.Error "Unsupported barrier"
+  end.
+
+Definition run_tlbi (tid : nat) (iis : IIS.t) (ts : TState.t) (tlbi : TLBI) :
+  Exec.t string (IIS.t * TState.t * Memory.t) :=
+  Exec.fail_if (tlbi.(TLBI_shareability) =? Shareability_NSH)
+    "Non-shareable TLBIs are not supported";;
+  Exec.fail_if (negb (tlbi.(TLBI_rec).(TLBIRecord_regime) =? Regime_EL10))
+    "TLBIs in other regimes than EL10 are unsupported";;
+  let asid := tlbi.(TLBI_rec).(TLBIRecord_asid) in
+  let last := tlbi.(TLBI_rec).(TLBIRecord_level) =? TLBILevel_Last in
+  let va := bv_extract 12 36 (tlbi.(TLBI_rec).(TLBIRecord_address)) in
+  let vpre := ts.(TState.vcse) ⊔ ts.(TState.vdsb) ⊔ ((*iio*) IIS.nreg iis)
+              ⊔ ((* ad-hoc data dep *) IIS.regs iis) in
+  let tlbiev :=
+    match tlbi.(TLBI_rec).(TLBIRecord_op) with
+    | TLBIOp_ALL => ()
+    | TLBIOp_ASID => ()
+    | TLBIOp_VAA => ()
+    | TLBIOp_VA => ()
+    | _ => ()
+    end
+  in Exec.Error "TODO".
+
+
+
+
+
+(** Runs an outcome. *)
+Definition run_outcome {A} (tid : nat) (o : outcome A) (iis : IIS.t)
+           (ts : TState.t) (init : Memory.initial) (mem : Memory.t)
+  : Exec.t string (IIS.t * TState.t * Memory.t * A) :=
+  let deps_to_view :=
+    fun deps => IIS.from_DepOn_opt deps ts iis in
+  match o with
+  | RegWrite reg direct deps val => Exec.Error "TODO"
+  | RegRead reg direct => Exec.Error "TODO"
+  | MemRead 8 rr =>
+      '(ts, iis, val) ← run_mem_read rr iis ts init mem;
+      Exec.ret (iis, ts, mem, inl (val, None))
+  | MemRead 4 rr => (* ifetch *)
+      opcode ← run_mem_read4 rr iis ts init mem;
+      Exec.ret (iis, ts, mem, inl (opcode, None))
+  | MemRead _ _ => Exec.Error "Memory read of size other than 8 or 4"
+  | MemWrite 8 wr =>
+      addr ← Exec.error_none "PA not supported" $ Loc.from_pa wr.(WriteReq.pa);
+      let vaddr := deps_to_view wr.(WriteReq.addr_dep_on) in
+      let data := wr.(WriteReq.value) in
+      let vdata := deps_to_view wr.(WriteReq.data_dep_on) in
+      let viio := IIS.nreg iis in
+      match wr.(WriteReq.access_kind) with
+      | AK_explicit eak =>
+          '(ts, mem) ← write_mem_xcl tid addr vaddr vdata viio eak ts mem data;
+          Exec.ret (iis, ts, mem, inl None)
+      | AK_ifetch () => Exec.Error "Write of type ifetch ???"
+      | AK_ttw () => Exec.Error "Write of type TTW ???"
+      | _ => Exec.Error "Unsupported non-explicit write"
+      end
+  | MemWrite _ _ => Exec.Error "Memory write of size other than 8"
+  | BranchAnnounce _ deps =>
+      let ts := TState.update TState.vspec (deps_to_view deps) ts in
+      Exec.ret (iis, ts, mem, ())
+  | Barrier barrier =>
+      '(iis, ts) ← run_barrier iis ts barrier;
+      Exec.ret (iis, ts, mem, ())
+  | TlbOp tlbi =>
+      '(iis, ts, mem) ← run_tlbi tid iis ts tlbi;
+      Exec.ret (iis, ts, mem, ())
+  | GenericFail s => Exec.Error ("Instruction failure: " ++ s)%string
+  | Choose n =>
+      v ← Exec.choose (bv n);
+      Exec.ret(iis, ts, mem, v)
+  | Discard => Exec.discard
+  | _ => Exec.Error "Unsupported outcome"
+  end.
+
+
+(** Runs an instruction monad object run_outcome as the effect handler *)
+Fixpoint run_iMon {A : Type} (i : iMon A) (iis : IIS.t) (tid : nat)
+         (ts : TState.t) (init : Memory.initial) (mem : Memory.t)
+  : Exec.t string (TState.t * Memory.t * A) :=
+  match i with
+  | Ret a => Exec.ret (ts, mem, a)
+  | Next o next =>
+      '(iis, ts, mem, res) ← run_outcome tid o iis ts init mem;
+      run_iMon (next res) iis tid ts init mem
+  end.
+
+(*** Implement GenPromising ***)
+
+Section PromStruct.
+  Context (isem : iSem).
+
+  Definition tState' : Type := TState.t * isem.(isa_state).
+
+  Definition tState_init' (tid : nat) (mem : memoryMap) (regs : registerMap)
+      : tState':=
+    (TState.init mem regs, isem.(init_state) tid).
+
+  Definition tState_nopromises' (tstate : tState') :=
+    tstate.1.(TState.prom) |> is_emptyb.
+
+  Local Notation pThread := (PThread.t tState' Ev.t).
+
+(** Run an iSem on a pThread  *)
+  Definition run_pthread (pthread : pThread) : Exec.t string pThread :=
+    let imon := isem.(semantic) pthread.(PThread.tstate).2 in
+    let initmem := pthread.(PThread.initmem) |> Memory.initial_from_memMap in
+    '(ts, mem, isa_st) ←@{Exec.t string}
+      run_iMon
+        imon
+        IIS.init
+        pthread.(PThread.tid)
+        pthread.(PThread.tstate).1
+        initmem
+        pthread.(PThread.events);
+    pthread |> setv PThread.tstate (ts, isa_st)
+            |> setv PThread.events mem
+            |> Exec.ret.
+
+
+  (* A thread is allowed to promise any promises with the correct tid.
+    This a non-certified promising model *)
+  Definition allowed_promises_nocert (pthread : pThread) :=
+    fun ev => Ev.tid ev = pthread.(PThread.tid).
+  Arguments allowed_promises_nocert _ _ /.
+
+  Definition emit_promise' (pthread : pThread) (ev : Ev.t) : tState' :=
+    let vev := length pthread.(PThread.events) in
+    pthread.(PThread.tstate) |> set fst (TState.promise vev).
+
+  Definition memory_snapshot' (memMap : memoryMap) (mem : Memory.t) : memoryMap :=
+    Memory.to_memMap (Memory.initial_from_memMap memMap) mem.
+
+  Definition UMPromising_nocert' : PromisingModel isem :=
+    {|tState := tState';
+      tState_init := tState_init';
+      tState_regs := TState.reg_map ∘ fst;
+      tState_isa_state := fun x => x.2;
+      tState_nopromises := tState_nopromises';
+      mEvent := Ev.t;
+      run_instr := run_pthread;
+      allowed_promises := allowed_promises_nocert;
+      emit_promise := emit_promise';
+      memory_snapshot := memory_snapshot';
+    |}.
+
+  Definition UMPromising_nocert := Promising_to_Modelnc UMPromising_nocert'.
+
+End PromStruct.
+Arguments allowed_promises_nocert _ _ _ /.
